Added sections to commute.v (#22)
* (Re)defined consistency

* Redefined decision as function (instead of relation).

* Cleaned up some stuff.

* Completed merge.

* Final clean-up

* Removed some unnecessary explicit arguments.

* Added Sections to commute.v

* nit.

commute.v
@@ -11,159 +11,135 @@ Class consensus_values :=
     about_C : exists (c1 c2 : C), c1 <> c2;
   }.
 
-Definition decision {message} (S : LSM_sig message) {CV : consensus_values} : Type
+Definition decision {message} (S : LSM_sig message) {CV : consensus_values}
   := @state _ S -> option C.
 
-(* 3.2.1 Decision finality *)
-(* Program Definition prot_state0 `{VLSM} : protocol_state := 
-  exist protocol_state_prop (proj1_sig s0) _.
-Next Obligation.
-  red.
-  exists None. 
-  constructor.
-Defined. *)
+Section CommuteSingleton.
+  
+  Context 
+    {message : Type}
+    {S : LSM_sig message}
+    {CV : consensus_values}
+    (V : VLSM S).
 
-Definition final {message} {S : LSM_sig message} (V : @VLSM message S) {CV : consensus_values}
-  : decision S -> Prop :=
-  fun (D : decision S) => forall (tr : protocol_trace V), 
-      forall (n1 n2 : nat) (s1 s2 : state) (c1 c2 : C),
-        (trace_nth (proj1_sig tr) n1 = Some s1) ->
-        (trace_nth (proj1_sig tr) n2 = Some s2) ->
-        (D s1 = (Some c1)) ->
-        (D s2 = (Some c2)) ->
-        c1 = c2.
+  (* 3.2.1 Decision finality *)
+  (* Program Definition prot_state0 `{VLSM} : protocol_state := 
+    exist protocol_state_prop (proj1_sig s0) _.
+  Next Obligation.
+    red.
+    exists None. 
+    constructor.
+  Defined. *)
 
-(* 3.2.2 Decision consistency *)
+  Definition final : decision S -> Prop :=
+    fun (D : decision S) => forall (tr : protocol_trace V), 
+        forall (n1 n2 : nat) (s1 s2 : state) (c1 c2 : C),
+          (trace_nth (proj1_sig tr) n1 = Some s1) ->
+          (trace_nth (proj1_sig tr) n2 = Some s2) ->
+          (D s1 = (Some c1)) ->
+          (D s2 = (Some c2)) ->
+          c1 = c2.
 
-Definition consistent
-  {CV : consensus_values}
-  {index : Set} `{Heqd : EqDec index}
-  {message : Type} 
-  {IS : index -> LSM_sig message}
-  (IM : forall i : index, @VLSM message (IS i))
-  (Hi : index)
-  (constraint : indexed_label IS -> indexed_state IS * option (indexed_proto_message IS) -> Prop)
-  (X := indexed_vlsm_constrained Hi IS IM constraint)
-  (ID : forall i : index, decision (IS i)) : Prop
-  :=
-    forall (tr : @protocol_trace _ _ X), 
-    forall (n1 n2 : nat),
-    forall (j k : index),
-    forall (s1 s2 : @state _ (sign X)),
-    forall (c1 c2 : C),
-    j <> k ->
-    trace_nth (proj1_sig tr) n1 = (Some s1) ->
-    trace_nth (proj1_sig tr) n2 = (Some s2) ->
-    (ID j) (@s1 j) = (Some c1) -> 
-    (ID k) (@s2 k) = (Some c2) -> 
-    c1 = c2.
+  (* 3.3.1 Initial protocol state bivalence *)
+  Definition bivalent : decision S -> Prop :=
+    fun (D : decision S) =>
+      (* All initial states decide on None *) 
+      (forall (s0 : state),
+        initial_state_prop s0 ->
+        D s0 = None) /\
+      (* Every protocol trace (already beginning from an initial state) contains a state deciding on each consensus value *) 
+      (forall (c : C) ,
+          exists (tr : protocol_trace V) (s : state) (n : nat), 
+            (trace_nth (proj1_sig tr) n) = Some s /\ D s = (Some c)).
 
-(** The following is an attempt to include finality in the definition of consistency by dropping the requirement 
-    that (j <> k). **)
+  (* 3.3.2 No stuck states *) 
 
-Definition final_and_consistent
-  {CV : consensus_values}
-  {index : Set} `{Heqd : EqDec index}
-  {message : Type} 
-  {IS : index -> LSM_sig message}
-  (IM : forall i : index, @VLSM message (IS i))
-  (Hi : index)
-  (constraint : indexed_label IS -> indexed_state IS * option (indexed_proto_message IS) -> Prop)
-  (X := indexed_vlsm_constrained Hi IS IM constraint)
-  (ID : forall i : index, decision (IS i)) : Prop
-  :=
-    forall (tr : @protocol_trace _ _ X), 
-    forall (n1 n2 : nat),
-    forall (j k : index),
-    forall (s1 s2 : @state _ (sign X)),
-    forall (c1 c2 : C),
-    trace_nth (proj1_sig tr) n1 = (Some s1) ->
-    trace_nth (proj1_sig tr) n2 = (Some s2) ->
-    (ID j) (@s1 j) = (Some c1) -> 
-    (ID k) (@s2 k) = (Some c2) -> 
-    c1 = c2.
+  Definition stuck_free : decision S -> Prop :=
+    fun (D : decision S) =>
+      (forall (s : state),
+          exists (tr : protocol_trace V) 
+                 (decided_state : state)
+                 (n_s n_decided : nat)
+                 (c : C),
+         trace_nth (proj1_sig tr) n_s = Some s /\
+         trace_nth (proj1_sig tr) n_decided = Some decided_state /\
+         n_decided >= n_s /\
+         D decided_state = Some c).
 
-Lemma final_and_consistent_implies_final
-  {CV : consensus_values}
-  {index : Set} `{Heqd : EqDec index}
-  {message : Type} 
-  {IS : index -> LSM_sig message}
-  (IM : forall i : index, @VLSM message (IS i))
-  (Hi : index)
-  (constraint : indexed_label IS -> indexed_state IS * option (indexed_proto_message IS) -> Prop)
-  (X := indexed_vlsm_constrained Hi IS IM constraint)
-  (ID : forall i : index, decision (IS i))
-  : 
-    final_and_consistent IM Hi constraint ID ->
-    forall i : index, final (indexed_vlsm_constrained_projection Hi IS IM constraint i) (ID i).
+  (* 3.3.3 Protocol definition symmetry *) 
+  (* How do we formalize this property set-theoretically? *)
 
-Proof.
-  unfold final_and_consistent.
-  intros.
-  unfold final.
-  intros.
-  Admitted.
+  Definition behavior : decision S -> Prop := 
+    fun _ => True.
 
-(* 3.3.1 Initial protocol state bivalence *)
-Definition bivalent {message} {S : LSM_sig message} (V : @VLSM message S) {CV : consensus_values} : decision S -> Prop :=
-  fun (D : decision S) =>
-    (* All initial states decide on None *) 
-    (forall (s0 : state),
-      initial_state_prop s0 ->
-      D s0 = None) /\
-    (* Every protocol trace (already beginning from an initial state) contains a state deciding on each consensus value *) 
-    (forall (c : C) ,
-        exists (tr : protocol_trace V) (s : state) (n : nat), 
-          (trace_nth (proj1_sig tr) n) = Some s /\ D s = (Some c)).
+  Definition symmetric : decision S -> Prop :=
+    fun (D : decision S) =>
+    exists (f : decision S -> decision S),
+      behavior D = behavior (f D).
 
-(* 3.3.2 No stuck states *) 
+End CommuteSingleton.
 
-Definition stuck_free {message} {S : LSM_sig message} (V : @VLSM message S) {CV : consensus_values} : decision S -> Prop :=
-  fun (D : decision S) =>
-    (forall (s : state),
-        exists (tr : protocol_trace V) 
-               (decided_state : state)
-               (n_s n_decided : nat)
-               (c : C),
-       trace_nth (proj1_sig tr) n_s = Some s /\
-       trace_nth (proj1_sig tr) n_decided = Some decided_state /\
-       n_decided >= n_s /\
-       D decided_state = Some c).
- 
-(* 3.3.3 Protocol definition symmetry *) 
-(* How do we formalize this property set-theoretically? *)
+Section CommuteIndexed.
 
-Definition behavior 
-  {message} 
-  {S : LSM_sig message} 
-  {V : @VLSM message S} 
-  {CV : consensus_values} : decision S -> Prop := 
-  fun _ => True.
+  Context
+    {CV : consensus_values}
+    {index : Set} `{Heqd : EqDec index}
+    {message : Type} 
+    {IS : index -> LSM_sig message}
+    (IM : forall i : index, VLSM (IS i))
+    (Hi : index)
+    (constraint : indexed_label IS -> indexed_state IS * option (indexed_proto_message IS) -> Prop)
+    (X := indexed_vlsm_constrained Hi IS IM constraint)
+    (ID : forall i : index, decision (IS i)).
+    
+  (* 3.2.2 Decision consistency *)
 
-Definition symmetric 
-  {message}
-  {S : LSM_sig message}
-  (V : @VLSM message S)
-  {CV : consensus_values} : decision S -> Prop :=
-  fun (D : decision S) =>
-  exists (f : decision S -> decision S),
-    behavior D = behavior (f D).
+  Definition consistent :=
+      forall (tr : protocol_trace X), 
+      forall (n1 n2 : nat),
+      forall (j k : index),
+      forall (s1 s2 : @state _ (sign X)),
+      forall (c1 c2 : C),
+      j <> k ->
+      trace_nth (proj1_sig tr) n1 = (Some s1) ->
+      trace_nth (proj1_sig tr) n2 = (Some s2) ->
+      (ID j) (s1 j) = (Some c1) -> 
+      (ID k) (s2 k) = (Some c2) -> 
+      c1 = c2.
 
-Definition live 
-  {CV : consensus_values}
-  {index : Set} `{Heqd : EqDec index}
-  {message : Type} 
-  {IS : index -> LSM_sig message}
-  (IM : forall i : index, @VLSM message (IS i))
-  (Hi : index)
-  (constraint : indexed_label IS -> indexed_state IS * option (indexed_proto_message IS) -> Prop)
-  (X := indexed_vlsm_constrained Hi IS IM constraint)
-  (ID : forall i : index, decision (IS i)) : Prop
-  :=
-  forall (tr : @protocol_trace _ _ X),
-    @complete_trace_prop _ _ _ _ _ X tr -> 
-    exists (s : @state _ (sign X)) (n : nat) (i : index) (c : C), 
-      trace_nth (proj1_sig tr) n = Some s /\
-      (ID i) (@s i) = Some c.
+  (** The following is an attempt to include finality in the definition of consistency by dropping the requirement 
+      that (j <> k). **)
+
+  Definition final_and_consistent : Prop :=
+      forall (tr : protocol_trace X), 
+      forall (n1 n2 : nat),
+      forall (j k : index),
+      forall (s1 s2 : @state _ (sign X)),
+      forall (c1 c2 : C),
+      trace_nth (proj1_sig tr) n1 = (Some s1) ->
+      trace_nth (proj1_sig tr) n2 = (Some s2) ->
+      (ID j) (s1 j) = (Some c1) -> 
+      (ID k) (s2 k) = (Some c2) -> 
+      c1 = c2.
+
+  Lemma final_and_consistent_implies_final : 
+      final_and_consistent ->
+      forall i : index, final (indexed_vlsm_constrained_projection Hi IS IM constraint i) (ID i).
+
+  Proof.
+    unfold final_and_consistent.
+    intros.
+    unfold final.
+    intros.
+    Admitted.
+
+  Definition live :=
+    forall (tr : protocol_trace X),
+      complete_trace_prop X tr -> 
+      exists (s : @state _ (sign X)) (n : nat) (i : index) (c : C), 
+        trace_nth (proj1_sig tr) n = Some s /\
+        (ID i) (s i) = Some c.
+
+End CommuteIndexed.
 
 (* Section 4 *)
