vlsm.v
@@ -455,7 +455,7 @@ we define states and messages together as a property over a product type. *)
            | Infinite s ls => False
            end.
 
-      Definition complete_trace_prop `{VLSM} (tr : protocol_trace) : Prop
+      Definition complete_trace_prop (tr : protocol_trace) : Prop
          := 
             match (proj1_sig tr) with 
             | Finite s ls => terminating_trace_prop (proj1_sig tr)
